Completed refactoring.

.Makefile.d
@@ -1,12 +1,18 @@
-src/Stm.vo src/Stm.glob src/Stm.v.beautified src/Stm.required_vo: src/Stm.v 
-src/Stm.vio: src/Stm.v 
-src/Stm.vos src/Stm.vok src/Stm.required_vos: src/Stm.v 
-src/Step.vo src/Step.glob src/Step.v.beautified src/Step.required_vo: src/Step.v src/Stm.vo
-src/Step.vio: src/Step.v src/Stm.vio
-src/Step.vos src/Step.vok src/Step.required_vos: src/Step.v src/Stm.vos
-src/Seq.vo src/Seq.glob src/Seq.v.beautified src/Seq.required_vo: src/Seq.v 
-src/Seq.vio: src/Seq.v 
-src/Seq.vos src/Seq.vok src/Seq.required_vos: src/Seq.v 
-src/Path.vo src/Path.glob src/Path.v.beautified src/Path.required_vo: src/Path.v 
-src/Path.vio: src/Path.v 
-src/Path.vos src/Path.vok src/Path.required_vos: src/Path.v 
+src/Sem.vo src/Sem.glob src/Sem.v.beautified src/Sem.required_vo: src/Sem.v 
+src/Sem.vio: src/Sem.v 
+src/Sem.vos src/Sem.vok src/Sem.required_vos: src/Sem.v 
+src/Enumerable.vo src/Enumerable.glob src/Enumerable.v.beautified src/Enumerable.required_vo: src/Enumerable.v src/Sem.vo
+src/Enumerable.vio: src/Enumerable.v src/Sem.vio
+src/Enumerable.vos src/Enumerable.vok src/Enumerable.required_vos: src/Enumerable.v src/Sem.vos
+src/Stm.vo src/Stm.glob src/Stm.v.beautified src/Stm.required_vo: src/Stm.v src/Sem.vo
+src/Stm.vio: src/Stm.v src/Sem.vio
+src/Stm.vos src/Stm.vok src/Stm.required_vos: src/Stm.v src/Sem.vos
+src/Step.vo src/Step.glob src/Step.v.beautified src/Step.required_vo: src/Step.v src/Stm.vo src/Sem.vo
+src/Step.vio: src/Step.v src/Stm.vio src/Sem.vio
+src/Step.vos src/Step.vok src/Step.required_vos: src/Step.v src/Stm.vos src/Sem.vos
+src/Path.vo src/Path.glob src/Path.v.beautified src/Path.required_vo: src/Path.v src/Stm.vo src/Step.vo src/Sem.vo
+src/Path.vio: src/Path.v src/Stm.vio src/Step.vio src/Sem.vio
+src/Path.vos src/Path.vok src/Path.required_vos: src/Path.v src/Stm.vos src/Step.vos src/Sem.vos
+src/Seq.vo src/Seq.glob src/Seq.v.beautified src/Seq.required_vo: src/Seq.v src/Stm.vo src/Step.vo
+src/Seq.vio: src/Seq.v src/Stm.vio src/Step.vio
+src/Seq.vos src/Seq.vok src/Seq.required_vos: src/Seq.v src/Stm.vos src/Step.vos
