src/Enumerable.v
@@ -1,0 +1,80 @@
+From Coq Require Import Lists.List.
+Import ListNotations.
+
+Class Enumerable (A : Type) :=
+  { enumerated : list A;
+    enumerated_all : forall x : A, In x enumerated;
+    enumerated_unique : NoDup enumerated }.
+
+From STM Require Import Sem.
+Section Example.
+
+  Definition Sem_enumerated : list Sem := [Green ; Yellow ; Red ; Black].
+
+  Theorem Sem_enumerated_all : forall s : Sem, In s Sem_enumerated.
+  Proof.
+    unfold Sem_enumerated.
+    destruct s.
+    - simpl. left. reflexivity.
+    - simpl. right. left. reflexivity.
+    - simpl. right. right. left. reflexivity.
+    - simpl. right. right. right. left. reflexivity.
+  Qed.
+
+  Theorem Sem_enumerated_unique : NoDup Sem_enumerated.
+  Proof.
+    unfold Sem_enumerated.
+    apply NoDup_cons.
+    - intro H. simpl in H. destruct H as [H | [H | [H | H]]].
+      + discriminate.
+      + discriminate.
+      + discriminate.
+      + contradiction.
+    - apply NoDup_cons.
+      + intro H. simpl in H. destruct H as [H | [H | H]].
+        * discriminate.
+        * discriminate.
+        * contradiction.
+      + apply NoDup_cons.
+        * intro H. simpl in H. destruct H as [H | H].
+          -- discriminate.
+          -- contradiction.
+        * apply NoDup_cons.
+          -- intro H. simpl in H. apply H.
+          -- apply NoDup_nil.
+  Qed.
+
+  Instance Sem_enumerable : Enumerable Sem :=
+    { enumerated := Sem_enumerated;
+      enumerated_all := Sem_enumerated_all;
+      enumerated_unique := Sem_enumerated_unique }.
+
+  Definition Ev_enumerated : list Ev := [Stop ; Next ; Fail].
+
+  Theorem Ev_enumerated_all : forall e : Ev, In e Ev_enumerated.
+  Proof.
+    unfold Ev_enumerated.
+    destruct e.
+    - simpl. left. reflexivity.
+    - simpl. right. left. reflexivity.
+    - simpl. right. right. left. reflexivity.
+  Qed.
+
+  Theorem Ev_enumerated_unique : NoDup Ev_enumerated.
+  Proof.
+    unfold Ev_enumerated.
+    apply NoDup_cons.
+    - intro H. simpl in H. destruct H as [H | [H | H]].
+      + discriminate.
+      + discriminate.
+      + contradiction.
+    -  apply NoDup_cons.
+       + intro H. simpl in H. destruct H as [H | H].
+         * discriminate.
+         * contradiction.
+      + apply NoDup_cons.
+         * intro H. simpl in H. apply H.
+         * apply NoDup_nil.
+  Qed.
+
+End Example.
