src/Path.v
@@ -3,9 +3,9 @@ From STM Require Import Step.
 
 (* State machine path definition *)
 Inductive Path S E (tr : Trans S E) (stm : Stm tr) : S -> S -> Prop :=
-| path_singl (ps1 : S) (ps2 : S) (stp : Step tr ps1 ps2)
+| path_singl (ps1 ps2 : S) (stp : Step tr ps1 ps2)
   : Path S E tr stm ps1 ps2
-| path_next (ps1 : S) (ps2 : S) (ps3 : S) (path : Path S E tr stm ps1 ps2)
+| path_next (ps1 ps2 ps3 : S) (path : Path S E tr stm ps1 ps2)
     (stp : Step tr ps2 ps3) : Path S E tr stm ps1 ps3.
 
 Arguments Path {S} {E} _ {stm}.
@@ -14,8 +14,8 @@ Arguments path_next {S} {E} _ {stm}.
 
 (* State machine path theorems *)
 
-Theorem path_extend_before : forall {S} {E} (tr : Trans S E) {stm : Stm tr}
-                                    (ss : S) (ss' : S) (es : S),
+Theorem path_extend_before : forall {S E} (tr : Trans S E) {stm : Stm tr}
+                                    (ss ss' es : S),
     Path tr ss es -> Step tr ss' ss -> Path tr ss' es.
 Proof.
   intros S E tr stm ss ss' es H1 H2.
@@ -28,8 +28,8 @@ Proof.
     + apply stp.
 Qed.
 
-Theorem path_extend_after : forall {S} {E} (tr : Trans S E) {stm : Stm tr}
-                                   (ss : S) (es : S) (es' : S),
+Theorem path_extend_after : forall {S E} (tr : Trans S E) {stm : Stm tr}
+                                   (ss es es' : S),
     Path tr ss es -> Step tr es es' -> Path tr ss es'.
 Proof.
   intros S E tr stm ss es es' H1 H2.
@@ -38,8 +38,8 @@ Proof.
   - apply H2.
 Qed.
 
-Theorem path_join : forall {S} {E} (tr : Trans S E) {stm : Stm tr}
-                           (ss : S) (ms : S) (es : S),
+Theorem path_join : forall {S E} (tr : Trans S E) {stm : Stm tr}
+                           (ss ms es : S),
     Path tr ss ms -> Path tr ms es -> Path tr ss es.
   intros S E tr stm ss ms es H1 H2.
   induction H2.
@@ -51,8 +51,8 @@ Theorem path_join : forall {S} {E} (tr : Trans S E) {stm : Stm tr}
     + apply stp.
 Qed.
 
-Theorem path_split : forall {S} {E} (tr : Trans S E) {stm : Stm tr}
-                            (ss : S) (es : S),
+Theorem path_split : forall {S E} (tr : Trans S E) {stm : Stm tr}
+                            (ss es : S),
     Path tr ss es -> ~(Step tr ss es) ->
     exists ms : S, Path tr ss ms /\ Path tr ms es.
 Proof.
@@ -65,8 +65,8 @@ Proof.
     + apply path_singl. apply stp.
 Qed.
 
-Theorem path_reduce_start : forall {S} {E} (tr : Trans S E) {stm : Stm tr}
-                                   (ss : S) (es : S),
+Theorem path_reduce_start : forall {S E} (tr : Trans S E) {stm : Stm tr}
+                                   (ss es : S),
     Path tr ss es -> ~(Step tr ss es) ->
     exists ss' : S, Step tr ss ss' -> Path tr ss' es.
 Proof.
@@ -76,8 +76,8 @@ Proof.
   - exists ps2. intros _. apply path_singl. apply stp.
 Qed.
 
-Theorem path_reduce_end : forall {S} {E} (tr : Trans S E) {stm : Stm tr}
-                                   (ss : S) (es : S),
+Theorem path_reduce_end : forall {S E} (tr : Trans S E) {stm : Stm tr}
+                                   (ss es : S),
     Path tr ss es -> ~(Step tr ss es) ->
     exists es' : S, Step tr es' es -> Path tr ss es'.
 Proof.
@@ -88,6 +88,7 @@ Proof.
 Qed.
 
 
+From STM Require Import Sem.
 Section Example.
 
   Theorem sem_path_ex1 : Path SemTrans Green Red.
@@ -112,29 +113,3 @@ Section Example.
   Qed.
 
 End Example.
-
-
-
-(* (* State sequence and path theorems *) *)
-
-(* Theorem seq_from_path : forall S E (stm : Stm S E) (ss : S) (es : S), *)
-(*     Path stm ss es -> exists l : list S, Seq stm (es :: l ++ [ss]). *)
-(* Proof. *)
-(*   intros S E stm ss es H. *)
-(*   induction H. *)
-(*   - exists []. simpl. apply seq_next. *)
-(*     + apply seq_one. *)
-(*     + apply psprf. *)
-(*   - destruct IHPath as [l' IHPath']. *)
-(*     exists (ps2 :: l'). *)
-(*     simpl. *)
-(*     apply (seq_extend_after _ _ _ _ ps2 ps3) in IHPath'. *)
-(*     + apply IHPath'. *)
-(*     + apply sprf. *)
-(* Qed. *)
-
-(* Theorem path_from_seq : forall S E (stm : Stm S E) (ss : S) (es : S) *)
-(*                                (l : list S), *)
-(*     Seq stm (es :: l ++ [ss]) -> Path stm ss es. *)
-(* Proof. *)
-(* Admitted. *)
