src/Sem.v
@@ -1,0 +1,14 @@
+Section Example.
+
+  Inductive Sem : Set :=
+  | Green
+  | Yellow
+  | Red
+  | Black.
+
+  Inductive Ev : Set :=
+  | Stop
+  | Next
+  | Fail.
+
+End Example.
